utils.dfy
@@ -1,0 +1,37 @@
+include "Node.dfy"
+
+function IndexOf(s: seq<Node>, e: Node) : int
+  requires e in s
+  requires NoDupes(s)
+  ensures 0 <= IndexOf(s,e) < |s|
+  ensures s[IndexOf(s,e)] == e
+{
+  var i :| 0 <= i < |s| && s[i] == e;
+  i
+}
+
+function get_next_seq_idx(s: seq<Node>, i: int): int
+  requires 0 <= i < |s|
+  requires NoDupes(s)
+  ensures 0 <= get_next_seq_idx(s,i) < |s|
+{
+  if |s| == 1 then 0
+  else
+    (i+1) % |s|
+}
+
+function get_prev_seq_idx(s: seq<Node>, i: int): int
+  requires 0 <= i < |s|
+  requires NoDupes(s)
+  ensures 0 <= get_prev_seq_idx(s, i) < |s|
+{
+  if |s| == 1 then 0
+  else
+    (i+|s|-1) % |s|
+}
+
+predicate NoDupes(a: seq<Node>) {
+  (forall i, j :: 0 <= i < |a| && 0 <= j < |a| && i != j ==> a[i] != a[j])
+  // for any integer in existence := i, j -> constraint => 0 <= i < len(a), j I!=J => A[I] = A[J]
+  // while loop => recursion / forall lemma
+}
